Hilbert10Experimental.lean
@@ -44,6 +44,7 @@ import Hilbert10Experimental.Spike.DecLoopDioph
 import Hilbert10Experimental.Spike.Sequences
 import Hilbert10Experimental.Spike.SelectorMask
 import Hilbert10Experimental.Spike.SelectorSlice
+import Hilbert10Experimental.Spike.SelectorSliceDioph
 
 /-!
 # Staging area
